Add support for Blake2b/Blake2s optimized versions in EverCrypt.Hash

code/hash/Hacl.Hash.Blake2.fst
@@ -235,8 +235,14 @@ let mk_update_last_ a m update_multi blake2_update_last_block s ev prev_len inpu
 let update_multi_blake2s_32 =
   mk_update_multi Blake2S Core.M32 update_blake2s_32
 
+let update_multi_blake2s_128 =
+  mk_update_multi Blake2S Core.M128 update_blake2s_128
+
 let update_multi_blake2b_32 =
   mk_update_multi Blake2B Core.M32 update_blake2b_32
+
+let update_multi_blake2b_256 =
+  mk_update_multi Blake2B Core.M256 update_blake2b_256
 
 let mk_update_last a m update_multi =
   mk_update_last_ a m update_multi (mk_blake2_update_last_block a m)
@@ -245,9 +251,17 @@ let update_last_blake2s_32 =
   mk_update_last_ Blake2S Core.M32 update_multi_blake2s_32
                   (mk_blake2_update_last_block Blake2S Core.M32)
 
+let update_last_blake2s_128 =
+  mk_update_last_ Blake2S Core.M128 update_multi_blake2s_128
+                  (mk_blake2_update_last_block Blake2S Core.M128)
+
 let update_last_blake2b_32 =
   mk_update_last_ Blake2B Core.M32 update_multi_blake2b_32
                   (mk_blake2_update_last_block Blake2B Core.M32)
+
+let update_last_blake2b_256 =
+  mk_update_last_ Blake2B Core.M256 update_multi_blake2b_256
+                  (mk_blake2_update_last_block Blake2B Core.M256)
 
 let mk_hash a m blake2 = fun input input_len dst ->
   let h0 = ST.get() in
@@ -259,4 +273,6 @@ let mk_hash a m blake2 = fun input input_len dst ->
   lemma_blake2_hash_equivalence a (B.as_seq h0 input)
 
 let hash_blake2s_32: hash_st Blake2S = mk_hash Blake2S Core.M32 Hacl.Blake2s_32.blake2s
+let hash_blake2s_128: hash_st Blake2S = mk_hash Blake2S Core.M128 Hacl.Blake2s_128.blake2s
 let hash_blake2b_32: hash_st Blake2B = mk_hash Blake2B Core.M32 Hacl.Blake2b_32.blake2b
+let hash_blake2b_256: hash_st Blake2B = mk_hash Blake2B Core.M256 Hacl.Blake2b_256.blake2b
